Added implementation of full optimality certification, and extracted stream-based checker.

checker/cOption.ml
@@ -4,6 +4,7 @@ let modules = ref []
 let tracefile = ref None
 let litfile = ref None
 let solfile = ref None
+let objective = ref None
 
 let verbosity = ref 0
 
@@ -47,6 +48,10 @@ let (speclist:(Arg.key * Arg.spec * Arg.doc) list) =
      ("-lits",
       Arg.String(fun f -> litfile := Some f),
       " mapping of trace literals to model semantics."
+     );
+     ("-objective",
+      Arg.String(fun s -> objective := Some s),
+      " variable to minimize."
      );
      ("-solution",
       Arg.String(fun f -> solfile := Some f),
