checker/certcp_stream.ml
@@ -1,0 +1,209 @@
+(* Top-level checker code. *)
+module List = ExtLib.List
+module A = DynArray
+module L = List
+module H = Hashtbl
+module GL = Genlex
+module MT = MTypes
+module C = Checker
+module Sol = SolCheck
+module M = Model
+module S = Spec
+module P = Parse
+module Pr = ProofState
+module C_impl = Checker_impl
+
+type ident = Pr.ident
+type ivar = int
+
+let ident_list = S.listof S.ident
+let int_list = S.listof S.intconst
+
+(*
+type arith =
+  | Mul of (ivar * (ivar * ivar))
+  | Div of (ivar * (ivar * ivar))
+*)
+
+(* Boolean variables are just integers with range [0, 1]. *)
+let print_list ?sep:(sep=";") f fmt xs =
+  Format.fprintf fmt "[@[" ;
+  begin
+    match xs with
+    | [] -> ()
+    | (h :: tl) ->
+      begin
+        f fmt h ;
+        List.iter (fun x ->
+          Format.fprintf fmt "%s@ " sep ;
+          f fmt x
+        ) tl
+      end
+  end ;
+  Format.fprintf fmt "]@]"
+
+let fmt = Format.std_formatter
+let err_fmt = Format.err_formatter
+(* let debug_print str = Format.fprintf fmt str *)
+let debug_print str = ()
+  
+let string_of_token = function
+  | GL.Kwd s -> s
+  | GL.Ident id -> id
+  | GL.Int x -> string_of_int x
+  | _ -> "<tok>"
+
+let chomp tokens token =
+  let next = Stream.next tokens in
+  if next <> token then
+    begin
+      Format.fprintf fmt "Parse error: expected %s, got %s." (string_of_token token) (string_of_token next) ;
+      failwith "Parse error"
+    end
+
+let parse_ilist =
+  let rec aux ls = parser
+    | [< 'GL.Int 0 >] -> List.rev ls
+    | [< 'GL.Kwd "-" ; 'GL.Int k ; ret = aux ((-k) :: ls) >] -> ret
+    | [< 'GL.Int k ; ret = aux (k :: ls) >] -> ret in
+ fun toks -> aux [] toks
+
+let parse_var_asg model = parser
+  | [< 'GL.Ident v ; 'GL.Kwd "=" ; 'GL.Int k >] ->
+      (M.get_ivar model v, k)
+
+let parse_asg model tokens =
+  chomp tokens (GL.Kwd "[") ;
+  let asg = ref [] in
+  while Stream.peek tokens <> Some (GL.Kwd "]")
+  do
+    asg := (parse_var_asg model tokens) :: !asg ;
+    (if Stream.peek tokens = Some (GL.Kwd ",") then
+      Stream.junk tokens)
+  done ;
+  List.rev !asg
+
+let check_inferences model_info lmap toks =
+  let model = Pr.model_of_model_info model_info in
+  let hint = ref (-1) in
+  while Stream.peek toks <> None
+  do
+    match Pr.parse_step model_info lmap toks
+    with
+    | C_impl.Intro (id, cl) ->
+        if not (C_impl.check_inference_model model !hint cl) then
+          Format.fprintf fmt "Inference failed.@."
+    | C_impl.Hint h -> hint := h
+    | C_impl.Resolve _ -> ()
+    | C_impl.Del _ -> ()
+  done
+
+let check_resolution model_info lmap toks =
+  let clause_db = H.create 17 in
+  let okay = ref true in
+  while !okay && Stream.peek toks <> None
+  do
+    match Pr.parse_step model_info lmap toks
+    with
+    | C_impl.Intro (id, cl) -> H.add clause_db id cl
+    | C_impl.Hint _ -> ()
+    | C_impl.Resolve (id, cl, ant_ids) ->
+      let ants = List.rev @@ List.map (H.find clause_db) ant_ids in
+      if not (C_impl.resolvable cl ants) then
+        begin
+          Format.fprintf fmt "@[Resolution failure:@ %d@ " id ;
+          Pr.print_clause fmt cl ;
+          Format.fprintf fmt "@ -/|@ " ;
+          print_list Format.pp_print_int fmt ant_ids ;
+          Format.fprintf fmt "@]@." ;
+          Format.open_box 2 ;
+          print_list Pr.print_clause fmt ants ;
+          Format.fprintf fmt "@]@.";
+          okay := false
+        end
+      else
+        H.add clause_db id cl
+    | C_impl.Del id -> H.remove clause_db id
+  done
+
+let main () =
+  (* Parse the command-line arguments *)
+  Arg.parse
+    COption.speclist
+      (begin fun infile -> COption.infile := Some infile end)
+      "check_cp <options> <model_file>"
+  ;
+  (* Parse the model specification *)
+  Builtins.register () ;
+  let model_channel = match !COption.infile with
+      | None -> stdin
+      | Some file -> open_in file
+  in
+  (* Register any additional checker modules. *)
+  debug_print "{Reading model..." ;
+  let tokens = Spec.lexer (Stream.of_channel model_channel) in 
+  let model_info = Pr.parse_model_info tokens in
+  (* let model = Pr.model_of_model_info model_info in *)
+  debug_print "done.}@." ;
+  (* Read the solution, if one provided. *)
+  let opt_sol = match !COption.solfile with
+    | None -> None
+    | Some sf ->
+      let asg_toks = Spec.lexer (Stream.of_channel (open_in sf)) in
+      Some (Pr.parse_solution model_info asg_toks)
+  in
+  (* Read the literal semantics . *)
+  debug_print "{Reading literals..." ;
+  let lit_tokens = match !COption.litfile with
+    | None -> tokens
+    | Some lfile -> Spec.lexer (Stream.of_channel (open_in lfile))
+  in
+  let lmap = Pr.parse_lit_map model_info lit_tokens in
+  debug_print "done.}@." ;
+  let model = Pr.model_of_model_info model_info in
+  match (!COption.objective, opt_sol, !COption.tracefile) with
+  | (Some ovar, Some sol, Some tfile) ->
+    let tchannel = open_in tfile in
+    let ttoks = (Spec.lexer (Stream.of_channel tchannel)) in
+    let obj = Pr.get_ivar model_info ovar in
+    let step0 = Pr.create model_info lmap ttoks in
+    let next_step = Pr.next in
+    begin
+      Format.fprintf fmt "Checking optimality...@." ;
+      let okay = C_impl.certify_optimal model obj sol max_int step0 next_step in
+      if okay then
+        Format.fprintf fmt "@ successful.@."
+      else
+        Format.fprintf fmt "@ failed.@."
+    end
+  | (None, Some sol, Some tfile) ->
+    Format.fprintf fmt "ERROR: Solution and trace provided, but no objective.@."
+  | (_, Some sol, _) ->
+    begin
+      Format.fprintf fmt "Checking solution...@." ;
+      let okay = C_impl.certify_solution model sol in
+      if okay then
+        Format.fprintf fmt "@ successful.@."
+      else
+        Format.fprintf fmt "@ failed.@."
+    end
+  | (_, _, Some tfile) ->
+    begin
+      let tchannel = open_in tfile in
+      (* let ttoks = Spec.lexer (Stream.of_channel tchannel) in *)
+      let ttoks = (Spec.lexer (Stream.of_channel tchannel)) in
+      (* check_inferences model_info lmap ttoks *)
+      (* check_resolution model_info lmap ttoks *)
+      (* *)
+      let step0 = Pr.create model_info lmap ttoks in
+      let next_step = Pr.next in
+      Format.fprintf fmt "Checking unsatisfiability...@." ;
+      let okay = C_impl.certify_unsat model max_int step0 next_step in
+      if okay then
+        Format.fprintf fmt "@ successful.@."
+      else
+        Format.fprintf fmt "@ failed.@."
+    end
+  | _ -> Format.fprintf fmt "ERROR: No solution or trace specified.@."
+
+let _ = main () 
