checker/coq/checker_impl.v
@@ -18,32 +18,34 @@ Set Extraction Optimize.
 Extraction "checker_impl.ml"
   sol.asg_of_alist
   prim.check_inf prim.check_clause
-  (* domain.check_tauto *)
+  
   domain.check_tauto_bnd
   domset.bounds_domset
   domset.check_tauto_dbnd
-  (*
-  cumulative.check_cumul
-  cumulative.check_cumul_tt
-  *)
+  
   cumulative.check_cumul_sol
   cumulative.check_cumul_bnd
   cumulative.check_cumul_tt_bnd
   cumul_dset.check_cumul_tt_dbnd
   reif.check_reif
-  (* linear.check_lincon *)
+  
   linear.check_lincon_sol
   linear.check_linear_bnd
   linear_dset.check_linear_dbnd
   linear_dset.check_reif_linear_dbnd
-  (* element.check_element *)
+  
   element.check_element_bnd
   element_dset.check_elem_dbnd
   element_dset.check_reif_elem_dbnd
+
   model.cst
   model.make_linear
   model.make_cumul
   model.make_element
+  resolution.resolvable
   log.certify_unsat
+  log.certify_optimal
+  log.check_inference_model
+
   nat_of_int int_of_nat.
 
